Getting rid of noind in s_up_set definition

relations.v
@@ -1,5 +1,5 @@
 From Coq Require Import Lia.
-From Coq Require Import Relations Program.Basics.
+From Coq Require Import Relations Relation_Operators Program.Basics.
 From mathcomp Require Import ssreflect ssrbool eqtype ssrfun seq order.
 From Equations Require Import Equations.
 From event_struct Require Import utilities wftype.
@@ -14,7 +14,7 @@ Local Open Scope order_scope.
 Section well_founded.
 
 Definition sfrel {T : eqType} (f : T -> seq T) : rel T :=
-  [rel a b | b \in f a].
+  [rel a b | a \in f b].
 
 Definition filter_neq {T : eqType} (f : T -> seq T) : T -> seq T :=
   fun n => filter^~ (f n) (fun x => x != n).
@@ -30,79 +30,63 @@ Hypothesis descend : forall x n, x \in f n -> x <= n.
 Lemma filter_lt n k : k \in f\eq n -> k < n.
 Proof. by rewrite mem_filter lt_neqAle => /andP[] -> /descend ->. Qed.
 
-Lemma rel_sublt a b : (sfrel f\eq) a b -> b < a.
+Lemma rel_sublt a b : (sfrel f\eq) a b -> a < b.
 Proof. rewrite/sfrel /=. exact: filter_lt. Qed.
+
+Definition hack n (g : forall x : T, x < n -> seq T) := 
+  let ys := f\eq n in 
+  let ps := flatten (map^~ ys (fun x => 
+  if x \in ys =P true is ReflectT pf then
+    g x (filter_lt _ _ pf)
+  else
+    [::]
+)) in ys ++ ps.
+
+Arguments hack /.
 
 (* Computation of the strict upward set of a given element
  * w.r.t relation R derived from function `f`,
  * i.e. s_up_set(x) = { y | x R y } 
  *)
-Equations(noind) s_up_set (n : T) : seq T by wf n (<%O : rel T) :=
-  s_up_set n := 
-    let ys := f\eq n in 
-    let ps := flatten (map^~ ys (fun x => 
-      if x \in ys =P true is ReflectT pf then
-        s_up_set x
-      else 
-        [::]
-    )) in
-    ys ++ ps.
-Next Obligation. exact: filter_lt. Qed.
+Equations s_up_set (n : T) : seq T by wf n (<%O : rel T) :=
+  s_up_set n := hack n s_up_set.
 
-Definition t_closure (a b : T) : bool := b \in s_up_set a.
+Definition t_closure (a b : T) : bool := a \in s_up_set b.
 
-Lemma ext_s_up_set (x : T) (g h : forall y : T, y < x -> seq T) :
-  (forall (y : T) (p : y < x), g y p = h y p) ->
-    s_up_set_functional x g = s_up_set_functional x h.
-Proof.
-  move=> H. rewrite /s_up_set_functional. apply/eqP.
-  rewrite eqseq_cat //=. apply/andP. split=> //=. apply/eqP.
-  congr flatten. apply/eq_in_map => y /filter_lt. by case: eqP.
-Qed.
-
-Lemma t_closure_lt a b : t_closure a b -> b < a.
-Proof.
-  move: a b. apply: wf_ind => a IH b.
-  rewrite /t_closure /s_up_set /Subterm.FixWf Fix_eq; last exact: ext_s_up_set.
-  rewrite {1}/s_up_set_functional mem_cat => /orP [/filter_lt //|].
-  case/flatten_mapP=> x /filter_lt xinf.
-  case: eqP => // /filter_lt /IH /apply ax. 
-  by apply: lt_trans; first apply: ax.
-Qed.
-
-Lemma clos_trans_lt a b : clos_trans_n1 T (sfrel f\eq) a b -> b < a.
+Lemma clos_trans_lt a b : clos_trans_n1 T (sfrel f\eq) a b -> a < b.
 Proof.
   rewrite/sfrel /=.
   elim=> [x /filter_lt // | x y xfy acx ax].
-  apply: lt_trans; last by apply: ax.
+  apply: lt_trans; first exact: ax.
   exact: filter_lt.
-Qed. 
+Qed.
+
+Notation step := (@tn1_trans T (sfrel f\eq) _ _ _).
+Notation base := (@tn1_step T (sfrel f\eq) _).
 
 (* Transitive closure reflection lemma *)
 Lemma t_closureP a b : 
-  reflect (clos_trans_1n T (sfrel f\eq) a b) (t_closure a b).
+  reflect (clos_trans_n1 T (sfrel f\eq) a b) (t_closure a b).
 Proof.
-  rewrite /t_closure.
-  move: a b. apply: wf_ind=> a IH b.
-  apply /(iffP idP).
-  { rewrite /s_up_set /Subterm.FixWf Fix_eq; last exact: ext_s_up_set.
-    rewrite {1}/s_up_set_functional mem_cat => /orP [].
-    { by constructor. }
-    case/flatten_mapP=> x xinf. case: eqP=> //=.
-    move=> /filter_lt /IH /apply H.
-    apply: Relation_Operators.t1n_trans; last exact H.
-    exact: xinf. }
-  move=> ctab. move: ctab IH. case.
-  { rewrite /sfrel /= => c afc IH.
-    rewrite /s_up_set /Subterm.FixWf Fix_eq; last exact: ext_s_up_set.
-    by rewrite {1}/s_up_set_functional mem_cat afc. }
-  rewrite /sfrel /= => c d cfd ctac IHd.
-  rewrite /s_up_set /Subterm.FixWf Fix_eq; last exact: ext_s_up_set.
-  rewrite {1}/s_up_set_functional mem_cat. apply/orP.
-  right. apply/flatten_mapP. exists c=> //=. case: eqP=> //= _.
-  apply/IHd=> //=. exact: filter_lt.
+  rewrite /t_closure. funelim (s_up_set b)=> /=. 
+  apply /(iffP idP); rewrite mem_cat /sfrel /=.
+  { move=> /orP[/base|/flatten_mapP[x]] //.
+    by case: eqP=> // S /filter_lt/X/(_ a x erefl) /apply /(step S). }
+  move: X=> /swap[[?->//|y ? /dup ? /filter_lt L /swap /(_ _ L a y erefl)]].
+  move=> /apply ?; apply/orP; right; apply/flatten_mapP.
+  exists y=> //. by case eqP.
 Qed.
 
+Lemma t_closure_lt a b : t_closure a b -> a < b.
+Proof. by move=> /t_closureP /clos_trans_lt. Qed.
+
+Lemma t_closure_trans : transitive t_closure.
+Proof.
+  move=> b a c /t_closureP ab /t_closureP bc.
+  apply /t_closureP /clos_trans_tn1 /t_trans.
+  { apply /clos_tn1_trans /ab. }
+  exact: clos_tn1_trans.
+Qed.
 
 (* Computation of the (non-strict) upward set of a given element
  * w.r.t relation R derived from function `f`,
@@ -110,11 +94,11 @@ Qed.
  *)
 Definition up_set a := a :: s_up_set a.
 
-Definition rt_closure a b := b \in up_set a. 
+Definition rt_closure a b := a \in up_set b. 
 
 (* Reflexive-transitive closure reflection lemma *)
 Lemma rt_closureP a b :
-  reflect (clos_refl_trans_1n T (sfrel f) a b) (rt_closure a b).
+  reflect (clos_refl_trans_n1 T (sfrel f) a b) (rt_closure a b).
 Proof.
   apply /(iffP idP).
   { rewrite /rt_closure. 
@@ -122,27 +106,25 @@ Proof.
     { constructor. }
     move: (t_closureP a b). 
     rewrite /t_closure => refl. move: (refl atb). 
-    elim=> [c d cfd | c d e cfd st rt].
-    { apply: Relation_Operators.rt1n_trans; last by constructor.
+    elim=> [c cfd | c d cfd st rt].
+    { apply: rtn1_trans; last by constructor.
       move: cfd. rewrite /sfrel /filter_neq //=.
       rewrite mem_filter. by move=> /andP [??]. }
-    apply: Relation_Operators.rt1n_trans; last exact: rt.
+    apply: rtn1_trans; last exact: rt.
     move: cfd. rewrite /sfrel /filter_neq //=.
     rewrite mem_filter. move=> /andP [? H]. exact: H. }
   move=> cab. rewrite /rt_closure /up_set.
   rewrite in_cons. apply/orP.
-  elim: cab => [| c d e st rt [/eqP -> | efd]]; first by left.
-  { case: (d =P c)=> [eq|neq] //=; first by left.
+  elim: cab => [| c d st rt [/eqP -> | efd]]; first by left.
+  { case: (c =P d)=> [eq| /eqP neq] //=; first by left.
     right. move: st. rewrite /sfrel /=.
-    rewrite /s_up_set /Subterm.FixWf Fix_eq; last by apply: ext_s_up_set.
-    rewrite {1}/s_up_set_functional mem_cat /filter_neq mem_filter => ->.
-     apply /orP. left. by apply /predD1P. }
-  case: (d =P c)=> [<-|neq] //=; first by right. 
-  right. move: (t_closureP d e)=> refl. move: (refl efd)=> ct.
-  apply /(t_closureP c e) /clos_trans_t1n /t_trans; first last.
-  { apply: clos_t1n_trans. exact: ct. }
-  apply: t_step. rewrite /sfrel /filter_neq //=. 
-  rewrite mem_filter. by apply /predD1P. 
+    funelim (s_up_set d) => cfn. rewrite /hack mem_cat. apply/orP. left.
+    by rewrite mem_filter cfn neq. }
+  case: (c =P d)=> [<-| /eqP neq] //=; first by right. 
+  right. move: (t_closureP a c)=> refl. move: (refl efd)=> ct.
+  apply /(t_closureP a d) /clos_trans_tn1 /t_trans.
+  { apply /clos_tn1_trans. exact: ct. }
+  apply: t_step. rewrite /sfrel /filter_neq //= mem_filter neq. exact: st.
 Qed.
 
 Lemma rt_closure_refl : reflexive rt_closure.
@@ -151,8 +133,8 @@ Proof. move=> a. exact: mem_head. Qed.
 Lemma rt_closure_trans : transitive rt_closure.
 Proof.
   move=> b a c /rt_closureP ab /rt_closureP bc.
-  apply/rt_closureP /clos_rt_rt1n /rt_trans.
-  apply/clos_rt1n_rt /ab. exact: clos_rt1n_rt.
+  apply/rt_closureP /clos_rt_rtn1 /rt_trans.
+  apply/clos_rtn1_rt /ab. exact: clos_rtn1_rt.
 Qed.
 
 End well_founded.
